temp/Spec.Claim.Map.fst
@@ -10,265 +10,266 @@ type kv (a: eqtype) (b:eqtype) =
 
 val equalKV: #a: eqtype -> #b: eqtype -> kv1: kv a b -> kv2:  kv a b -> Tot bool
 let equalKV #a #b kv1 kv2 = 
-    (kv1.key = kv2.key) && (kv1.value = kv2.value)
-    
+	(kv1.key = kv2.key) && (kv1.value = kv2.value)
+	
 
 
 type map (a: eqtype) (b:eqtype) = 
-    |MapCons: list (kv a b) -> map a b
-    |MapList: l1: list a -> l2: list b{length l1 = length l2} -> map a b 
+	|MapCons: list (kv a b) -> map a b
+	|MapList: l1: list a -> l2: list b{length l1 = length l2} -> map a b 
 
 val isMapCons: #a: eqtype -> #b: eqtype -> map a b -> bool
 let isMapCons #a #b m = 
-    match m with 
-    | MapCons _ -> true    
-    | MapList _ _ -> false    
+	match m with 
+	| MapCons _ -> true	
+	| MapList _ _ -> false	
 
 val isMapList: #a: eqtype -> #b: eqtype -> map a b -> bool
 let isMapList #a #b m = 
-    match m with 
-    | MapCons _ -> false    
-    | MapList _ _ -> true            
+	match m with 
+	| MapCons _ -> false	
+	| MapList _ _ -> true			
  
 val size: #a: eqtype -> #b: eqtype -> map a b -> nat
 let size #a #b map = 
-    match  map with
-    | MapCons lst -> length lst
-    | MapList l1 _-> length l1 
+	match  map with
+	| MapCons lst -> length lst
+	| MapList l1 _-> length l1 
 
 val isEmpty: #a: eqtype -> #b: eqtype -> map a b -> bool 
 let isEmpty #a #b map = size #a #b map = 0
 
 private val _containsKeyKV:#a: eqtype -> #b : eqtype ->  l: list (kv a b) -> element: a -> counter : int -> Tot int
 let rec _containsKeyKV #a #b l element counter = 
-    match l with 
-    | hd:: tl -> if hd.key = element then counter else _containsKeyKV tl element (counter+1)
-    | [] -> -1
+	match l with 
+	| hd:: tl -> if hd.key = element then counter else _containsKeyKV tl element (counter+1)
+	| [] -> -1
 
 private val _containsKey:#a: eqtype -> list a -> element : a -> counter: int-> Tot int
 let rec _containsKey #a l element counter = 
-    match l with 
-    |hd:: tl -> if hd = element then counter else _containsKey #a tl element (counter +1)
-    | [] -> -1
+	match l with 
+	|hd:: tl -> if hd = element then counter else _containsKey #a tl element (counter +1)
+	| [] -> -1
 
 val containsKey: #a: eqtype -> #b: eqtype -> map a b -> a -> bool
 let containsKey #a #b map key = 
-    match map with 
-    | MapCons lst -> let r =  _containsKeyKV lst key 0 in r > -1
-    | MapList l1 l2 -> let r = _containsKey l1 key 0 in r > -1
+	match map with 
+	| MapCons lst -> let r =  _containsKeyKV lst key 0 in r > -1
+	| MapList l1 l2 -> let r = _containsKey l1 key 0 in r > -1
 
 private val _containsValueKV: #a: eqtype -> #b: eqtype -> l: list (kv a b) -> element : b -> counter : int -> Tot int
 let rec _containsValueKV #a #b l element counter = 
-    match l with 
-    | hd::tl -> if hd.value = element then counter else _containsValueKV tl element (counter+1)
-    | [] -> -1
+	match l with 
+	| hd::tl -> if hd.value = element then counter else _containsValueKV tl element (counter+1)
+	| [] -> -1
 
 private val _containsValue:  #b: eqtype -> list b -> element : b -> counter: int-> Tot int
 let rec _containsValue #b l element counter = 
-    match l with 
-    |hd::tl -> if hd = element then counter else _containsValue #b tl element (counter+1)
-    |[] -> -1
+	match l with 
+	|hd::tl -> if hd = element then counter else _containsValue #b tl element (counter+1)
+	|[] -> -1
 
 val containsValue: #a: eqtype -> #b: eqtype -> map a b -> b -> bool
 let containsValue #a #b map value = 
-    match  map with
-    | MapCons lst  -> let r = _containsValueKV lst value 0 in r > -1
-    | MapList l1 l2     -> let r = _containsValue  #b l2 value 0 in r > -1
+	match  map with
+	| MapCons lst  -> let r = _containsValueKV lst value 0 in r > -1
+	| MapList l1 l2	 -> let r = _containsValue  #b l2 value 0 in r > -1
 
 val get: #a: eqtype -> #b: eqtype -> map a b -> key: a -> option b
 let get #a #b map key = 
-    match map with 
-    | MapCons lst -> let i = _containsKeyKV #a #b lst key 0 in 
-                        if (i > -1 && i < length lst) 
-                            then Some (FStar.List.Tot.index lst i).value
-                        else None
-    | MapList l1 l2 -> let i = _containsKey #a l1 key 0 in 
-                            if (i > -1 && i < length l2)
-                                then Some (FStar.List.Tot.index l2 i)
-                            else None                    
+	match map with 
+	| MapCons lst -> let i = _containsKeyKV #a #b lst key 0 in 
+						if (i > -1 && i < length lst) 
+							then Some (FStar.List.Tot.index lst i).value
+						else None
+	| MapList l1 l2 -> let i = _containsKey #a l1 key 0 in 
+							if (i > -1 && i < length l2)
+								then Some (FStar.List.Tot.index l2 i)
+							else None					
 
 val append_len: l1: list 'a -> l2: list 'a -> 
-            Lemma (ensures (length (append l1 l2) = length l1 + length l2))
+			Lemma (ensures (length (append l1 l2) = length l1 + length l2))
 
 let rec append_len l1 l2 = 
-    match l1 with 
-    | [] -> ()
-    | hd::tl -> append_len tl l2            
+	match l1 with 
+	| [] -> ()
+	| hd::tl -> append_len tl l2			
 
 val put: #a: eqtype -> #b: eqtype -> m: map a b -> e1: a -> e2: b -> 
-        Tot (r: map a b {isMapList m = isMapList r /\ isMapCons m = isMapCons r /\ size r = size m +1})
+		Tot (r: map a b {isMapList m = isMapList r /\ isMapCons m = isMapCons r /\ size r = size m +1})
 let put #a #b m e1 e2 = 
-    match m with 
-    |MapCons list -> let temp = MkKV e1 e2 in 
-                        append_len list [temp];
-                        MapCons (List.append list [temp])
-    |MapList l1 l2 -> assert (length l1 = length l2); 
-                      let l1_2 = append l1 [e1] in 
-                      append_len l1 [e1];
-                      assert(length l1_2 = (length l1 + 1));
-                      let l2_2 = append l2 [e2] in 
-                      append_len l2 [e2];
-                      assert(length l1_2  = length l2_2);
-                      MapList l1_2 l2_2
+	match m with 
+	|MapCons list -> let temp = MkKV e1 e2 in 
+						append_len list [temp];
+						MapCons (List.append list [temp])
+	|MapList l1 l2 -> assert (length l1 = length l2); 
+					  let l1_2 = append l1 [e1] in 
+					  append_len l1 [e1];
+					  assert(length l1_2 = (length l1 + 1));
+					  let l2_2 = append l2 [e2] in 
+					  append_len l2 [e2];
+					  assert(length l1_2  = length l2_2);
+					  MapList l1_2 l2_2
 
 val put2: #a: eqtype -> #b:eqtype -> m: map a b -> e: kv a b -> 
-    Tot(r: map a b {isMapList m = isMapList r /\ isMapCons m = isMapCons r /\ size r = size m + 1})
+	Tot(r: map a b {isMapList m = isMapList r /\ isMapCons m = isMapCons r /\ size r = size m + 1})
 let put2 #a #b m e = 
-    match m with 
-    |MapCons list -> append_len list [e];
-                        MapCons (List.append list [e])
-    |MapList l1 l2 -> let key = e.key in 
-                        let value = e.value in 
-                        let keys = append l1 [key] in 
-                        let values = append l2 [value] in 
-                        append_len l1 [key];
-                        append_len l2 [value];
-                        assert(length keys = length values);
-                        MapList keys values
+	match m with 
+	|MapCons list -> append_len list [e];
+						MapCons (List.append list [e])
+	|MapList l1 l2 -> let key = e.key in 
+						let value = e.value in 
+						let keys = append l1 [key] in 
+						let values = append l2 [value] in 
+						append_len l1 [key];
+						append_len l2 [value];
+						assert(length keys = length values);
+						MapList keys values
 
 (*)
 val _split_list: l: list 'a -> 
-        counter: nat -> 
-        index_finish: nat{index_finish < length l /\ counter < index_finish} -> l_temp: list 'a -> 
-        Tot (list 'a)(decreases (index_finish - counter))
+		counter: nat -> 
+		index_finish: nat{index_finish < length l /\ counter < index_finish} -> l_temp: list 'a -> 
+		Tot (list 'a)(decreases (index_finish - counter))
 let rec _split_list l counter index_finish l_temp = 
-    let element = index l counter in 
-    let l_temp = append l_temp [element] in 
-    if (counter +1 < index_finish)
-        then _split_list l (counter+1) index_finish l_temp
-    else l_temp
+	let element = index l counter in 
+	let l_temp = append l_temp [element] in 
+	if (counter +1 < index_finish)
+		then _split_list l (counter+1) index_finish l_temp
+	else l_temp
 *)
 
 assume val split_list: l: list 'a ->index_start: nat ->
-     index_finish : nat -> 
-     Tot (r:list 'a{length r = index_finish - index_start})
+	 index_finish : nat -> 
+	 Tot (r:list 'a{length r = index_finish - index_start})
 (*let split_list l index_start index_finish = 
-    let counter = index_start in 
-    _split_list l counter index_finish []
+	let counter = index_start in 
+	_split_list l counter index_finish []
 *)
 
 val remove: #a: eqtype -> #b: eqtype -> m: map a b -> a -> map a b
 let remove #a #b m key  = 
-    match m with 
-    | MapCons lst -> let i = _containsKeyKV #a #b lst key 0 in 
-                        if (i > -1 && i < length lst) 
-                            then 
-                                (
-                                    let lst_fst = split_list lst 0 i in 
-                                    let lst_snd = split_list lst i (length lst)  
-                                    in MapCons (append lst_fst lst_snd)
-                                )    
-                        else
-                            m        
-    | MapList l1 l2 -> m                        
+	match m with 
+	| MapCons lst -> let i = _containsKeyKV #a #b lst key 0 in 
+						if (i > -1 && i < length lst) 
+							then 
+								(
+									let lst_fst = split_list lst 0 i in 
+									let lst_snd = split_list lst i (length lst)  
+									in MapCons (append lst_fst lst_snd)
+								)	
+						else
+							m		
+	| MapList l1 l2 -> m						
 
 val putAll: #a: eqtype -> #b: eqtype -> m: map a b -> 
-            l: list (kv a b) -> Tot(r: map a b{size r = size m + length l /\
-                                        isMapList m = isMapList r /\ isMapCons m = isMapCons r})
-                                (decreases (length l))
+			l: list (kv a b) -> Tot(r: map a b{size r = size m + length l /\
+										isMapList m = isMapList r /\ isMapCons m = isMapCons r})
+								(decreases (length l))
 let rec putAll #a #b m lst = 
-    match lst with 
-    | hd::tl -> let m = put2 #a #b m hd in putAll #a #b m tl
-    | [] -> m
+	match lst with 
+	| hd::tl -> let m = put2 #a #b m hd in putAll #a #b m tl
+	| [] -> m
 
 val putAll2: #a: eqtype -> #b: eqtype -> m: map a b -> 
-            lstA: list a -> lstB: list b{length lstA = length lstB} -> 
-            Tot (r: map a b{size r = size m + length lstA /\ isMapList m = isMapList r /\ isMapCons m = isMapCons r})
-            (decreases (length lstA))
+			lstA: list a -> lstB: list b{length lstA = length lstB} -> 
+			Tot (r: map a b{size r = size m + length lstA /\ isMapList m = isMapList r /\ isMapCons m = isMapCons r})
+			(decreases (length lstA))
 
 let rec putAll2 #a #b m lstA lstB = 
-    match lstA with 
-    |hdA::tlA ->let m1 = put2 #a #b m (MkKV (hdA) (hd lstB)) in 
-                assert(length (tlA) =  length (tl lstB));
-                putAll2 #a #b m1 (tlA) (tl lstB)
-    |[] -> m            
+	match lstA with 
+	|hdA::tlA ->let m1 = put2 #a #b m (MkKV (hdA) (hd lstB)) in 
+				assert(length (tlA) =  length (tl lstB));
+				putAll2 #a #b m1 (tlA) (tl lstB)
+	|[] -> m			
 
 val clear: #a: eqtype -> #b: eqtype -> map a b -> map a b (*very important method, but for the commmon java sense *)
 let clear #a #b m = 
-    match m with 
-    | MapCons _ -> MapCons [] 
-    | MapList _ _ -> MapList [] []
+	match m with 
+	| MapCons _ -> MapCons [] 
+	| MapList _ _ -> MapList [] []
 
 val createEmptyC: #a: eqtype -> #b: eqtype ->Tot(m : map a b {isMapCons m= true/\ size m = 0})
 let createEmptyC #a #b = 
-    MapCons [] 
+	MapCons [] 
 
 val createEmptyL: #a: eqtype -> #b: eqtype -> Tot (m: map a b {isMapList m = true /\ size m = 0})
 let createEmptyL #a #b = 
-    MapList [] [] 
+	MapList [] [] 
 
 val keySet: #a: eqtype -> #b: eqtype -> m: map a b -> Tot(l: list a{length l = size m})
 let keySet #a #b m = 
-    match m with 
-    | MapCons lst -> FStar.List.Tot.map (fun (x: kv a b) -> x.key) lst
-    | MapList l1 _ -> l1
+	match m with 
+	| MapCons lst -> FStar.List.Tot.map (fun (x: kv a b) -> x.key) lst
+	| MapList l1 _ -> l1
 
 val values: #a: eqtype -> #b: eqtype -> m:map a b -> Tot(l: list b{length l = size m})
 let values #a #b m = 
-    match m with 
-    | MapCons lst -> FStar.List.Tot.map  (fun (x: kv a b) -> x.value) lst
-    | MapList _ l2 -> l2
+	match m with 
+	| MapCons lst -> FStar.List.Tot.map  (fun (x: kv a b) -> x.value) lst
+	| MapList _ l2 -> l2
 
 val _mapToMapList: #a: eqtype -> #b: eqtype -> m: map a b -> Tot(r: map a b{isMapList r = true /\ size m = size r})
 
 let _mapToMapList #a #b m = 
-    let keys = keySet #a #b m in 
-    let values = values #a #b m in 
-    assert(length keys = length values);
-    let map = createEmptyL #a #b in 
-    putAll2 #a #b map keys values 
+	let keys = keySet #a #b m in 
+	let values = values #a #b m in 
+	assert(length keys = length values);
+	let map = createEmptyL #a #b in 
+	putAll2 #a #b map keys values 
 
 val _mapToMapCons: #a: eqtype -> #b: eqtype -> m: map a b {size m >0} -> 
-        Tot(r: map a b {isMapCons r = true /\ size m = size r})
+		Tot(r: map a b {isMapCons r = true /\ size m = size r})
 
 let _mapToMapCons #a #b m = 
-    match m with 
-    | MapCons _ -> m 
-    | MapList l1 l2 -> 
-        let empty = createEmptyC #a #b in 
-        putAll2 #a #b empty l1 l2
+	match m with 
+	| MapCons _ -> m 
+	| MapList l1 l2 -> 
+		let empty = createEmptyC #a #b in 
+		putAll2 #a #b empty l1 l2
 
 val pairs: #a: eqtype-> #b: eqtype -> m: map a b{size m > 0} -> Tot (list (kv a b))
 let pairs #a #b m = 
-    match m with 
-    | MapCons lst -> lst 
-    | MapList _ _ ->    let newMap =  _mapToMapCons #a #b m in 
-                        match newMap with 
-                        MapCons lst -> lst
+	match m with 
+	| MapCons lst -> lst 
+	| MapList _ _ ->	let newMap =  _mapToMapCons #a #b m in 
+						match newMap with 
+						MapCons lst -> lst
 
 assume val sorted: #a: eqtype  -> (a -> a -> Tot bool) -> s:list a -> Tot bool (decreases (length s))
 
 assume val sort: #a: eqtype ->  l: list a ->f: (a -> a -> Tot bool){total_order a f} -> Tot (r: list a {sorted f r /\ length l = length r})
 
 val _equals: #a: eqtype -> #b: eqtype -> l1: list (kv a b) -> 
-    l2: list (kv a b){length l1 = length l2}-> counter: nat{counter < length l1} -> Tot bool (decreases (length l1 - counter))
+	l2: list (kv a b){length l1 = length l2}-> counter: nat{counter < length l1} -> Tot bool (decreases (length l1 - counter))
 
 let rec _equals #a #b l1 l2 counter = 
-    let e1 = index l1 counter in 
-    let e2 = index l2 counter in 
-    equalKV e1 e2 && 
-        (
-            if (counter + 1 < length l1) 
-                then _equals #a #b l1 l2 (counter+1) 
-            else true
-        )
+	let e1 = index l1 counter in 
+	let e2 = index l2 counter in 
+	equalKV e1 e2 && 
+		(
+			if (counter + 1 < length l1) 
+				then _equals #a #b l1 l2 (counter+1) 
+			else true
+		)
 
 val equals: #a: eqtype -> #b: eqtype -> 
-        m1: map a b -> m2: map a b {size m1 = size m2 /\ size m1 > 0} -> 
-        f:((kv a b) -> (kv a b) -> Tot bool){total_order (kv a b) f} -> bool
+		m1: map a b -> m2: map a b {size m1 = size m2 /\ size m1 > 0} -> 
+		f:((kv a b) -> (kv a b) -> Tot bool){total_order (kv a b) f} -> bool
 
 let equals #a #b m1 m2 f = 
-    let m1 = _mapToMapCons #a #b m1 in 
-    let m2 = _mapToMapCons #a #b m2 in 
-    let m1 = sort (match m1 with | MapCons lst -> lst) f in 
-    let m2 = sort (match m2 with | MapCons lst -> lst) f in 
-    assert(length m1 = length m2);
-    _equals #a #b m1 m2 0
+	let m1 = _mapToMapCons #a #b m1 in 
+	let m2 = _mapToMapCons #a #b m2 in 
+	let m1 = sort (match m1 with | MapCons lst -> lst) f in 
+	let m2 = sort (match m2 with | MapCons lst -> lst) f in 
+	assert(length m1 = length m2);
+	_equals #a #b m1 m2 0
 
 val index: #a: eqtype -> #b: eqtype -> m: map a b ->i : nat {i < size m} ->  kv a b 
 let index #a #b m i = 
-    match m with 
-    |MapCons lst -> index lst i
-    |MapList l1 l2 -> let key = index l1 i in 
-                        let value = index l2 i in 
-                        MkKV key value
+	match m with 
+	|MapCons lst -> index lst i
+	|MapList l1 l2 -> let key = index l1 i in 
+						let value = index l2 i in 
+						MkKV key value
+
